LeanSubst/Automation/Attributes.lean
@@ -1,0 +1,88 @@
+import Batteries.Lean.TagAttribute
+import Lean.Elab
+
+namespace LeanSubstAttributes
+
+  open Lean Elab Tactic Meta Command
+
+  initialize leanSubstVar : TagAttribute ← registerTagAttribute `_leansubst_var "Indicates that a constructor is a variable constructor."
+
+  #check Lean.Parser.Command.classAbbrev
+  #check Lean.Parser.Term.attrInstance
+  #check Attr.coe
+
+  #check Lean.Parser.Attr.simple
+
+  #check mkElabAttribute
+
+  syntax (name := leansubst_binder_attr) "_leansubst_binder" "[" term,* "]" "[" ident,* "]" "[" num,* "]" : attr
+
+  initialize leanSubstBinder : ParametricAttribute $ List (Term × Ident × Nat) ← registerParametricAttribute {
+    name := `leansubst_binder_attr,
+    descr := "Blah",
+    getParam := fun
+    | name, stx@`(attr| _leansubst_binder [ $closures,* ] [ $tys,* ] [ $ps,* ]) => do
+      let ret := Array.zip closures.getElems (Array.zip tys.getElems ps.getElems)
+      pure $ ret.toList.map (fun (a, b, c) => (a, b, c.getNat))
+    | _, _ => throwUnsupportedSyntax
+  }
+
+  initialize leanSubstBinder' : ParametricAttribute Nat ← registerParametricAttribute {
+    name := `leansubst_binder',
+    descr := "Blah",
+    getParam := fun
+    | name, stx@`(Lean.Parser.Attr.simple| $_ $n:num) => do
+      pure n.getNat
+    | name, stx@`(Lean.Parser.Term.attrInstance| $_) => do
+      dbg_trace s!"oh no {name}, {stx}"
+      pure 0
+  }
+
+  declare_syntax_cat bind_data (behavior := symbol)
+
+  syntax term &" of " term &" at " &" pos " num : bind_data
+
+  syntax term &" at " &" pos " num : bind_data
+
+  declare_syntax_cat bind_decl (behavior := symbol)
+
+  syntax " bind " bind_data,+ &" in " ident : bind_decl
+
+  elab "#leansubst" stx:bind_decl : command => stx |> fun
+  | `(bind_decl| bind $data:bind_data,* in $ctor) => do
+    let mapfun := fun
+    | `(bind_data| $closure:term of $ty:ident at pos $p) => pure (closure, ty, p)
+    | `(bind_data| $ty:ident at pos $p) => pure (Syntax.mkNatLit 1, ty, p)
+    | _ => throwUnsupportedSyntax
+    let data ← data.getElems.mapM mapfun
+    let closures := data.map (·.1)
+    let tys := data.map (·.2.1)
+    let ps : Array (TSyntax `num) := data.map (·.2.2)
+    elabCommand $ ← `(
+      attribute [_leansubst_binder [$closures,*] [$tys,*] [$ps,*]] $ctor
+    )
+  | _ => throwUnsupportedSyntax
+
+  declare_syntax_cat var_decl (behavior := symbol)
+
+  syntax " var " ident : var_decl
+
+  syntax " var " ident &" at " &" pos " num : var_decl
+
+  -- elab "#leansubst" stx:var_decl : command => stx |> fun
+  -- | `(var_decl| var $ctor at pos $n) => do
+  --   elabCommand $ ← `(
+  --     attribute [_leansubst_var $n] $ctor
+  --   )
+  -- |  `(var_decl| var $ctor) => do
+  --   elabCommand $ ← `(
+  --     attribute [_leansubst_var 0] $ctor
+  --   )
+  -- | _ => throwUnsupportedSyntax
+
+  elab "#leansubst" &" var " ctor:ident : command => do
+    elabCommand $ ← `(
+      attribute [_leansubst_var] $ctor
+    )
+
+end LeanSubstAttributes
