LeanSubst/Automation/Basic.lean
@@ -1,0 +1,582 @@
+import LeanSubst
+import Lean.Elab.Tactic
+import Lean.Elab.Term.TermElabM
+import LeanSubst.Automation.Attributes
+import Aesop
+
+namespace Automation
+  open Lean Elab Tactic Meta LeanSubst Command Aesop LeanSubstAttributes
+
+  def getConstructors (typeName : Name) : MetaM (List Name) := do
+    match (← getEnv).find? typeName with
+    | some (.inductInfo val) => return val.ctors
+    | _ => throwError "Could not get constructors of: {typeName}"
+
+  def isVar (ctor : Name) : MetaM Bool := do
+    pure $ leanSubstVar.hasTag (← getEnv) ctor
+
+  def isNotVar (ctor : Name) : MetaM Bool := do
+    pure $ ¬ leanSubstVar.hasTag (← getEnv) ctor
+
+  def getNonVarConstructors (typeName : Name) : MetaM (List Name) := do
+    match (← getEnv).find? typeName with
+    | some (.inductInfo val) => val.ctors.filterM isNotVar
+    | _ => throwError "Could not get constructors of: {typeName}"
+
+  def getVarCtor (type : Name) : MetaM (Option Name) := do
+    List.findM? (isVar) (← getConstructors type)
+
+  def getBinderParam (ctor : Name) : MetaM (Option Nat) := do
+    pure (leanSubstBinder'.getParam? (← getEnv) ctor)
+
+  def isBinder (ctor : Name) : MetaM Bool := do
+    if let some _ := ← getBinderParam ctor then pure true else pure false
+
+  def getBinderCtors (type : Name) : MetaM (List (Name × Nat)) := do
+    (← getConstructors type).filterMapM
+      (fun ctor ↦ do if let some i := ← getBinderParam ctor then pure $ some ⟨ctor, i⟩ else pure none)
+
+  def getNonTaggedCtors (type : Name) : MetaM (List Name) := do
+    List.filterM (fun n => do pure (¬ (← isVar n) ∧ ¬ (← isBinder n))) (← getConstructors type)
+
+  def mapFst {α β} (ℓ : List (α × β)) := ℓ.map Prod.fst
+
+  def mapSnd {α β} (ℓ : List (α × β)) := ℓ.map Prod.snd
+
+  -- We use this to get the types of all the arguments in a constructor
+  def getForallBinderTypes : Expr → List Expr
+  | .forallE _ t b _ => t :: getForallBinderTypes b
+  | _ => []
+
+  -- A lot of the metaprogramming stuff is replicated between rmap and smap, with minor changes here and there.
+  -- Therefore, we often write functions that take a MapType as a flag argument and produce the definition, theorem, etc.
+  inductive MapType
+  | rmap
+  | smap
+
+  -- Names of variables
+  def xN (n : Nat) : TSyntax `term := mkIdent (.mkStr1 $ s!"x{n}")
+  def xN' (n : Nat) : TSyntax `ident := mkIdent (.mkStr1 $ s!"x{n}")
+  def x := mkIdent `x
+  def y := mkIdent `y
+  def z := mkIdent `z
+  def r := mkIdent `r
+  def s := mkIdent `s
+  def n := mkIdent `n
+  def t := mkIdent `t
+  def σ := mkIdent `σ
+  def τ := mkIdent `τ
+
+  -- For each constructor argument in which something is bound, we need to keep track of how many of each thing is bound.
+  inductive ArgData
+  | binder : List (Term × Ident) → ArgData -- (Term × Ident) corresponds to ([num bound closure] × [type being bound])
+  | var
+  | none
+
+  -- The "closure" is a function that takes the arguments of the constructor and returns the number of bound variables.
+  def getClosureFromArgData (ty : Ident) : ArgData → Option Term
+  | .binder xs => (xs.find? (fun (_, ty') => BEq.beq ty' ty)).map (·.1)
+  | _ => none
+
+  def getCtorArgData (ctor : Name) (p : Nat) : CommandElabM $ ArgData := do
+    if let some data := leanSubstBinder.getParam? (← getEnv) ctor then
+      pure $ .binder $ data |> .filter (fun (_, _, p') => p' = p) |> .map (fun (t1, t2, _) => (t1, t2))
+    else if ← liftCoreM $ runMetaMAsCoreM $ isVar ctor then
+      pure .var
+    else
+      pure .none
+
+  def numArgsInCtor (ctor : Name) : CommandElabM Nat := do
+    let ctorType := (← getConstInfo ctor).type
+    let argTypes := getForallBinderTypes ctorType
+    pure $ argTypes.length
+
+  def isBoundInCtorAtPos (A Bctor : Name) (pos : Nat) : CommandElabM Bool := do
+    let data ← getCtorArgData Bctor pos
+    if let .binder binds := data then
+      binds.anyM (fun ⟨_, ty⟩ ↦ do liftCoreM $ runMetaMAsCoreM $ isDefEq (← liftTermElabM $ Term.elabTerm (mkIdent A) none) (← liftTermElabM $ Term.elabTerm ty none))
+    else
+      pure false
+
+  def isBoundInCtor (A Bctor : Name) : CommandElabM Bool := do
+    (List.range $ ← numArgsInCtor Bctor).anyM (fun pos ↦ isBoundInCtorAtPos A Bctor pos)
+
+  -- Check if A is bound in B
+  def isBoundIn (A B : Name) : CommandElabM Bool := do
+    (← liftCoreM $ runMetaMAsCoreM $ getConstructors B).anyM (isBoundInCtor A)
+
+  def mkCtorLhs (ctor : Name) : CommandElabM $ Term := do
+    let ctorType := (← getConstInfo ctor).type
+    let argTypes := getForallBinderTypes ctorType
+    let argTypesWithData ←
+      argTypes
+      |> (.zip · (List.range $ List.length argTypes))
+      |> List.mapM (fun (ty, p) ↦ do pure (ty, ← getCtorArgData ctor p, xN' p))
+    let xs : List Ident := argTypesWithData.map (fun (_, _, x) ↦ x)
+    `($(mkIdent ctor) $(xs.toArray)*)
+
+  def mkCtorArgs (ctor : Name) : CommandElabM $ List Ident := do
+    pure $ List.map xN' $ List.range $ (← numArgsInCtor ctor)
+
+  -- Applies f to each argument
+  def mkCtorRhs (f : Expr → ArgData → Ident → List Ident → CommandElabM Term) (ctor : Name) : CommandElabM $ Term := do
+    let ctorType := (← getConstInfo ctor).type
+    let argTypes := getForallBinderTypes ctorType
+    let argTypesWithData ←
+      argTypes
+      |> (.zip · (List.range $ List.length argTypes))
+      |> List.mapM (fun (ty, p) ↦ do pure (ty, ← getCtorArgData ctor p, xN' p))
+    let xs : List Ident := argTypesWithData.map (fun (_, _, x) ↦ x)
+    let mappedXs ← (argTypesWithData.toArray.mapM (fun (ty, data, x) ↦ (f ty data x xs)))
+    `($(mkIdent ctor) $mappedXs*)
+
+  def mkCtorCase (f : Expr → ArgData → Ident → List Ident → CommandElabM Term) (ctor : Name) : CommandElabM $ TSyntax `Lean.Parser.Term.matchAltExpr := do
+    let lhs ← mkCtorLhs ctor
+    let rhs ← mkCtorRhs f ctor
+    `(Parser.Term.matchAltExpr| | $lhs => $rhs)
+
+  def mkVarCtorRhs (f : List Ident → Term → CommandElabM Term) (ctor : Name) : CommandElabM $ Term := do
+    f (← mkCtorArgs ctor) $ mkIdent ctor
+
+  def mkVarCtorCase (f : List Ident → Term → CommandElabM Term) (ctor : Name) : CommandElabM $ TSyntax `Lean.Parser.Term.matchAltExpr := do
+    let lhs ← mkCtorLhs ctor
+    let rhs ← mkVarCtorRhs f ctor
+    `(Parser.Term.matchAltExpr| | $lhs => $rhs)
+
+  def mkCtorEq (fLhs : Term → CommandElabM Term) (fRhs : Expr → ArgData → Ident → List Ident → CommandElabM Term) (ctor : Name) (fVar : Option (List Ident → Term → CommandElabM Term) := none): CommandElabM $ Term := do
+    let lhs ← mkCtorLhs ctor >>= fLhs
+    let rhs ←
+      if ← liftCoreM $ runMetaMAsCoreM $ isVar ctor then
+        if let some fVar := fVar then mkVarCtorRhs fVar ctor else mkCtorRhs fRhs ctor
+      else
+        mkCtorRhs fRhs ctor
+    `($lhs = $rhs)
+
+  -- We need to give the option of handling the var case by doing more than just mapping each argument, hence the fVar argument here.
+  def mkAllCases (f : Expr → ArgData → Ident → List Ident → CommandElabM Term) (ty : Name) (fVar : Option (List Ident → Term → CommandElabM Term) := none) : CommandElabM $ TSyntaxArray `Lean.Parser.Term.matchAltExpr := do
+    if let some fVar := fVar then
+      let nonVarCtors ← liftCoreM $ runMetaMAsCoreM $ getNonVarConstructors ty
+      let nonVarCases ← nonVarCtors.toArray.mapM (mkCtorCase f)
+      if let some varCtor ← liftCoreM $ runMetaMAsCoreM $ getVarCtor ty then
+        let varCase ← mkVarCtorCase fVar varCtor
+        pure $ Array.append #[varCase] nonVarCases
+      else throwError "ruh roh"
+    else
+      let ctors ← liftCoreM $ runMetaMAsCoreM $ getConstructors ty
+      ctors.toArray.mapM (mkCtorCase f)
+
+  -- Given an RenVec or SubstVec, extracts the correctly-typed entry.
+  def getTy (rσ : Ident) (tys : Array Ident) (ty : Ident) : CommandElabM Term := do
+    let pos := tys.idxOf ty
+    let mut stx ← `($rσ)
+    for _ in List.range $ pos do
+      stx ← `($stx.2)
+    `($stx.1)
+
+  -- Applies a computation for each suffix in the list Tys.
+  def forEachSuffix : (tys : List Ident) → (f : List Ident → CommandElabM Unit) → CommandElabM Unit
+  | [], _ => pure ()
+  | tys@(.cons _ tys'), f => do
+    f tys
+    forEachSuffix tys' f
+
+  def forEachPrefix : (tys : List Ident) → (f : List Ident → CommandElabM Unit) → CommandElabM Unit
+  | [], _ => pure ()
+  | tys@(.cons _ _), f => do
+    f tys
+    forEachSuffix tys.reverse.tail.reverse f
+
+  def forHeadAndEachSuffix : (tys : List Ident) → (f : List Ident → CommandElabM Unit) → CommandElabM Unit
+  | [], _ => pure ()
+  | .cons ty [], f => do f [ty]
+  | tys@(.cons ty _), f => do
+    f [ty]
+    forEachSuffix tys f
+
+  def forEachCtor (ty : Name) (f : Name → CommandElabM Unit) : CommandElabM Unit := do
+    for ctor in ← liftCoreM $ runMetaMAsCoreM $ getConstructors ty do f ctor
+
+  def forEachTy (tys : List Ident) (f : Ident → CommandElabM Unit) : CommandElabM Unit := do
+    for ty in tys do f ty
+
+  -- We use this as a return value to indicate whether the returned term should be applied as a map or as a lift.
+  inductive MapOrLift
+  | map : Term → MapOrLift
+  | lift : Term → MapOrLift
+  | none : MapOrLift
+
+  -- The main function
+  def genTy (tys : List Ident) : CommandElabM Unit := do
+    let toGlobal (ty : Ident) : CommandElabM Name := Command.liftCoreM $ realizeGlobalConstNoOverload ty.raw
+    let ty := tys[0]!
+    let tyName := ty.raw.getId
+    let tyStr := tyName.toString
+    let tyNameGlobal ← toGlobal ty
+
+    dbg_trace s!"Generating {ty} with list {tys}"
+
+    let tyArr ← `([$tys.toArray,*])
+    let tysNamesGlobal ← tys.mapM toGlobal
+
+    let qualify str := mkIdent $ .str tyName str
+
+    let varCtorName ← liftCoreM $ runMetaMAsCoreM $ getVarCtor tyNameGlobal
+    let varName ← match varCtorName with
+    | some name => pure name
+    | none => throwError "ruh roh"
+    let varType := (← getConstInfo varName).type
+    let var := mkIdent varName
+
+    let from_action := qualify "from_action"
+    let from_action_id := qualify "from_action_id"
+    let from_action_succ := qualify "from_action_succ"
+    let from_action_re := qualify "from_action_re"
+    let from_action_su := qualify "from_action_su"
+    elabCommand $ ← `(
+      @[coe]
+      def $from_action : Action $ty → $ty
+      | re $y => $var $y
+      | su $t => $t
+
+      @[simp, grind =]
+      theorem $from_action_id {$n} : $from_action (𝐬0.act $n) = $var $n := rfl
+
+      @[simp, grind =]
+      theorem $from_action_succ {$n} : $from_action (𝐬1.act $n) = $var ($n + 1) := rfl
+
+      @[simp, grind =]
+      theorem $from_action_re {$n} : $from_action (re $n) = $var $n := rfl
+
+      @[simp, grind =]
+      theorem $from_action_su {$n} : $from_action (su $n) = $n := rfl
+
+      instance : Coe (Action $ty) $ty where
+        coe := $from_action
+    )
+
+
+    let rmap := qualify "rmap"
+    let smap := qualify "smap"
+
+    let mkMapSingletonInstance (mapType : MapType) (ty' : Ident) := do
+      let tyList ← (tys.map (TSyntax.raw ·)).mapM (fun `($ty'') ↦ do
+        let ty'Expr ← liftTermElabM $ Term.elabTerm ty' none
+        let ty''Expr ← liftTermElabM $ Term.elabTerm ty'' none
+        if ← liftCoreM $ runMetaMAsCoreM $ isDefEq ty'Expr ty''Expr then
+          match mapType with | .rmap => `($(r).1) | .smap => `($(σ).1)
+        else
+          match mapType with | .rmap => `(Ren.id $ty'') | .smap => `(Subst.id $ty''))
+      let tyArr := (tyList.append [← `(.nil)]).toArray
+      match mapType with
+      | .rmap =>
+        elabCommand $ ← `(
+          instance : RenMap $ty [$ty'] where
+            rmap $r:ident := $rmap ⟨ $tyArr:term,* ⟩
+        )
+      | .smap =>
+        elabCommand $ ← `(
+          instance : SubstMap $ty [$ty'] where
+            smap $σ:ident := $smap ⟨ $tyArr:term,* ⟩
+        )
+
+    let mkMapInstances (mapType : MapType) := do
+      match mapType with
+      | .rmap =>
+        elabCommand $ ← `(
+          instance : RenMap $ty [$tys.toArray,*] where
+            rmap := $rmap
+
+          instance : RenMap $ty [] where
+            rmap _ := id
+        )
+      | .smap =>
+        elabCommand $ ← `(
+          instance : SubstMap $ty [$tys.toArray,*] where
+            smap := $smap
+
+          instance : SubstMap $ty [] where
+            smap _ := id
+        )
+      -- If the length of `tys` is 1, then we've already done the only necessary RenMap
+      -- TODO: check, do we also need all prefixes here?
+      if tys.length > 1 then
+        forEachTy tys $ mkMapSingletonInstance mapType
+
+    let mkSuffixInstances (mapType : MapType) := do
+      let TheSuffix ← match mapType with | .rmap => ``(RenSuffix) | .smap => ``(SubstSuffix)
+      forEachSuffix tys.tail (fun sfx ↦ do
+        elabCommand $ ← `(
+          instance : $TheSuffix $ty:ident [$sfx.toArray,*] := ⟨⟩
+        )
+      )
+      elabCommand $ ← `(
+        instance : $TheSuffix $ty:ident [] := ⟨⟩
+      )
+
+    -- rmap setup
+    let getLiftsOfTy (data : ArgData) (xs : List Ident) (ty : Ident)  : CommandElabM $ Term := do
+      let closure := getClosureFromArgData ty data
+      if let some closure := closure then
+        let closureTypeExpr ← liftTermElabM $ inferType (← liftTermElabM $ Term.elabTerm closure none)
+        if closureTypeExpr.isForall || closureTypeExpr.isArrow then -- does .isForall subsume .isArrow?
+          let closureApp ← `(term| $closure $(xs.toArray)*)
+          let closureAppExpr ← liftTermElabM $ Term.elabTerm closureApp none
+          let closureAppExprReduced ← liftCoreM $ runMetaMAsCoreM $ reduce closureAppExpr
+          liftTermElabM closureAppExprReduced.toSyntax
+        else
+          pure closure
+      else
+        pure (Syntax.mkNatLit 0)
+
+    let mkLiftArr (data : ArgData) (xs : List Ident) (tys := tys) : CommandElabM $ Option Term :=
+      match data with
+      | .binder _ => do
+        let lifts ← tys.mapM $ getLiftsOfTy data xs
+        -- Check if all lifts are syntactically just 0
+        if List.all lifts (fun stx ↦ BEq.beq stx $ Syntax.mkNatLit 0) then
+          pure none
+        else
+          pure $ ← `([$lifts.toArray,*])
+      | _ => do
+        pure none
+
+    -- smap setup
+    let getIncrementsOfTy (lifts : List Term) (tysNamesGlobal : List Name) (ty : Name) : CommandElabM $ List (Ident × Term) := do
+      let tysLiftsZip := tysNamesGlobal.zip lifts
+      let increments : List (Ident × Term) ←
+        tysLiftsZip.mapM
+          (fun ⟨ty', lift⟩ ↦ do
+            -- Is there a better way to check if two names are equal?
+            let ty'_eq_ty ← liftCoreM $ runMetaMAsCoreM $ isDefEq (← liftTermElabM $ Term.elabTerm (mkIdent ty') none) (← liftTermElabM $ Term.elabTerm (mkIdent ty) none)
+            if ¬ ty'_eq_ty ∧ (← isBoundIn ty' ty) then
+              pure ⟨mkIdent ty', lift⟩
+            else
+              pure ⟨mkIdent ty', Syntax.mkNatLit 0⟩)
+      pure $ increments.filter (fun (_, stx) ↦ match stx with | `(0) => false | _ => true)
+
+    let mkMapArr (data : ArgData) (xs : List Ident) (tys : List Ident) : CommandElabM $ Option MapOrLift :=
+      match data with
+      | .binder _ => do
+        let lifts ← tys.mapM $ getLiftsOfTy data xs
+        let optionLifts := lifts.map (fun stx : Term ↦ if BEq.beq stx $ Syntax.mkNatLit 0 then none else some stx)
+        -- Check if all lifts are syntactically just 0
+        if optionLifts.all (fun | none => true | some _ => false) then
+          pure none
+        else
+          let tysNamesGlobal ← tys.mapM toGlobal
+          let incrementsList ← tysNamesGlobal.mapM $ getIncrementsOfTy lifts tysNamesGlobal
+          let zipped := incrementsList.zip optionLifts
+          let ops : List $ Term × Bool ← zipped.mapM (fun ⟨incs, lift⟩ ↦ do
+            let incOps ← incs.mapM (fun ⟨ty, inc⟩ ↦
+              if BEq.beq inc $ Syntax.mkNatLit 0 then `(Ren.id $ty:ident) else `(Ren.add $ty:ident $inc))
+            let anyIncs := incs.tail.any (fun ⟨_, inc⟩ ↦ ¬ (BEq.beq inc $ Syntax.mkNatLit 0))
+
+            let tyTail := tysNamesGlobal.tail.toArray.map mkIdent
+            let op ← match (anyIncs, lift) with
+            | (false, none) => `(.skip)
+            | (true, none) => `(.ren [$tyTail,*] ⟨$incOps.tail.toArray,*, .nil⟩)
+            | (false, some ℓ) => `(.lift $ℓ)
+            | (true, some ℓ) => `(.both [$tyTail,*] ⟨$incOps.tail.toArray,*, .nil⟩ $ℓ)
+            pure ⟨op, anyIncs⟩
+          )
+          if ops.all (¬ ·.2) then -- If we don't have to apply any renamings
+            pure $ MapOrLift.lift $ ← `([$lifts.toArray,*])
+          else
+            pure $ MapOrLift.map $ ← (ops.map Prod.fst).foldrM (fun t1 t2 ↦ `($t1 $ $t2)) $ ← `(LeanSubst.SubstVec.MapOps.nil)
+      | _ => pure none
+
+    let smap_fVar (tys : List Ident) xs ctor : CommandElabM Term := do
+      if (← liftCoreM $ runMetaMAsCoreM $ isDefEq (← liftTermElabM $ Term.elabTerm tys[0]!.raw none) (← liftTermElabM $ Term.elabTerm ty.raw none)) then
+        `($(σ).1.act $(xs[0]!):ident) -- TODO: At the moment, this doesn't generalize to vars with data
+      else
+        `($ctor $(xs[0]!):ident)
+
+    -- rmap/smap arg mapping function
+    let map_f (mapType : MapType) (useTCSyntax : Bool) ty' data (x : Ident) (xs : List Ident) (tys := tys) := match data with
+    | ArgData.var => do
+      match mapType with
+      | .rmap =>
+        if (← liftCoreM $ runMetaMAsCoreM $ isDefEq (← liftTermElabM $ Term.elabTerm tys[0]!.raw none) (← liftTermElabM $ Term.elabTerm ty.raw none)) then
+          `($(r).1.act $x) -- NOTE: assumes that the type being generated is the first type in [tys]
+        else
+          `($x)
+      | .smap => throwError "smap var case"
+    | _ => do
+      let tyExpr ← liftTermElabM $ Term.elabTerm ty none
+      if ← liftCoreM $ runMetaMAsCoreM $ isDefEq tyExpr ty' then
+        match mapType with
+        | .rmap =>
+          if let some liftArr ← mkLiftArr data xs (tys := tys) then
+            if useTCSyntax then `(($x)⟨$(r).lift $liftArr,⟩) else `($rmap ($(r).lift $liftArr) $x)
+          else
+            if useTCSyntax then `(($x)⟨$(r),⟩) else `($rmap $r $x)
+        | .smap =>
+          if let MapOrLift.map opsArr ← mkMapArr data xs tys then
+            if useTCSyntax then `(($x)[$(σ).map $opsArr,]) else `($smap ($(σ).map $opsArr) $x)
+          else if let MapOrLift.lift opsArr ← mkMapArr data xs tys then
+            if useTCSyntax then `(($x)[$(σ).lift $opsArr,]) else `($smap ($(σ).lift $opsArr) $x)
+          else
+            if useTCSyntax then `(($x)[$(σ),]) else `($smap $σ $x)
+      else if let some theTy ← List.findM? (fun (ty : Ident) ↦ do pure (← liftCoreM $ runMetaMAsCoreM $ isDefEq (← liftTermElabM $ Term.elabTerm ty.raw none) ty')) tys then
+        match mapType with
+        | .rmap =>
+          let r' ← getTy r tys.toArray theTy
+          `(($x⟨$r'⟩))
+        | .smap =>
+          let σ' ← getTy σ tys.toArray theTy
+          `(($x)[$σ'])
+      else
+        `($x)
+
+    -- theorems
+    let mkMapThms (mapType : MapType) := do
+      let mapStr := match mapType with | .rmap => "rmap" | .smap => "smap"
+      let rσ : Ident := match mapType with | .rmap => r | .smap => σ
+      let map := match mapType with | .rmap => rmap | .smap => smap
+      let map_fix := qualify s!"{mapStr}_fix"
+      let TheVec ← match mapType with | .rmap => ``(RenVec) | .smap => ``(SubstVec)
+
+      let eq ← match mapType with
+      | .rmap => `($map $rσ $t = $t⟨$rσ,⟩)
+      | .smap => `($map $rσ $t = $t[$rσ,])
+      let simp ← match mapType with | .rmap => `(by simp [RenMap.rmap]) | .smap => `(by simp [SubstMap.smap])
+      elabCommand $ ← `(
+        @[simp]
+        theorem $map_fix {$rσ : $TheVec [$tys.toArray,*]} {$t : $ty} : $eq := $simp
+      )
+
+      let map_empty := qualify s!"{mapStr}_empty"
+      let eq ← match mapType with | .rmap => `($t⟨$rσ,⟩ = $t) | .smap => `($t[$rσ,] = $t)
+      elabCommand $ ← `(
+        @[simp]
+        theorem $map_empty {$t : $ty} {$rσ : $TheVec []} : $eq := rfl
+      )
+
+      let proof ← match mapType with
+      | .rmap => `(by first | rfl | simp only [RenMap.rmap] ; rw [$rmap:ident] ; try simp | simp only [RenMap.rmap] ; simp ; aesop)
+      | .smap => `(by first | rfl | simp only [SubstMap.smap] ; rw [$smap:ident] ; try simp | simp only [SubstMap.smap] ; simp ; aesop)
+      forHeadAndEachSuffix tys (fun sfx ↦ forEachCtor tyNameGlobal (fun ctor ↦ do
+        let tyQual := if tys.length = 1 then "" else "_" ++ ("_".intercalate $ sfx.map (fun (ty : Ident) ↦ ty.raw.getId.toString.toLower))
+        let thmName := qualify s!"{mapStr}{tyQual}_{ctor.components.getLast!}"
+        let fRhs := map_f mapType true (tys := sfx)
+        let fLhs lhs : CommandElabM Term := match mapType with | .rmap => `(($lhs)⟨$(rσ),⟩) | .smap => `(($lhs)[$(rσ),])
+        let eq ← mkCtorEq fLhs fRhs ctor (fVar := match mapType with | .rmap => none | .smap => some $ smap_fVar sfx)
+        let args ← mkCtorArgs ctor
+        elabCommand $ ← `(
+          @[simp]
+          theorem $thmName {$args.toArray*} {$rσ : $TheVec [$sfx.toArray,*]} : $eq :=
+            $proof
+        )
+      ))
+
+    let mkFromActionMapThms (mapType : MapType) := do
+      let map := match mapType with | .rmap => "rmap" | .smap => "smap"
+      let from_action_map := qualify s!"from_action_{map}"
+      let rσ : Ident := match mapType with | .rmap => r | .smap => σ
+      let eq ← match mapType with
+      | .rmap => `(($from_action $t)⟨$rσ,⟩ = $from_action ($t⟨$rσ,⟩))
+      | .smap => `(($from_action $t)[$rσ,] = $from_action ($t[$rσ,]))
+      let TheVec ← match mapType with | .rmap => ``(RenVec) | .smap => ``(SubstVec)
+      elabCommand $ ← `(
+        @[simp]
+        theorem $from_action_map {$t : Action $ty} {$rσ : $TheVec [$tys.toArray,*]} : $eq := by
+          cases $t:ident <;> (first | rfl | simp | simp [$from_action:ident] | aesop)
+      )
+
+      let from_action_mapi (i : Nat) := qualify $ s!"from_action_{map}{i}"
+      if tys.length > 1 then
+        for i in List.range tys.length do
+          elabCommand $ ← `(
+            @[simp]
+            theorem $(from_action_mapi i) {$t : Action $ty} {$rσ : $TheVec [$(tys[i]!)]} : $eq := by
+              cases $t:ident <;> (first | rfl | simp | simp [$from_action:ident] | aesop)
+          )
+
+    let mkMapAllInstances (mapType : MapType) := do
+      let TheMapStr := match mapType with | .rmap => "RenMap" | .smap => "SubstMap"
+      let TheMapAll ← match mapType with | .rmap => ``(LeanSubst.RenMapAll) | .smap => ``(LeanSubst.SubstMapAll)
+      let instTheMapAll_ty := mkIdent $ .mkStr1 s!"inst{TheMapStr}All_{ty.raw.getId.toString}" -- not qualified
+      elabCommand $ ← `(
+        @[reducible, simp]
+        instance $instTheMapAll_ty:ident : $TheMapAll [$ty] := .cons .nil
+      )
+      if tys.length > 1 then
+        let tysPostfix := "_".intercalate (tys.map (fun (ty : Ident) ↦ ty.raw.getId.toString))
+        let tysPostfix' := "_".intercalate (tys.tail.map (fun (ty : Ident) ↦ ty.raw.getId.toString))
+        let instTheMapAll_tys := mkIdent $ .mkStr1 s!"inst{TheMapStr}All_{tysPostfix}" -- not qualified
+        let instTheMapAll_tys' := mkIdent $ .mkStr1 s!"inst{TheMapStr}All_{tysPostfix'}" -- not qualified
+        elabCommand $ ← `(
+          instance $instTheMapAll_tys:ident : $TheMapAll [$tys.toArray:ident,*] := .cons $instTheMapAll_tys'
+        )
+
+    -- Executing rmap stuff
+    let rmapCases ← mkAllCases (map_f .rmap false) tyNameGlobal
+    elabCommand $ ← `(
+      @[simp]
+      def $rmap ($r : RenVec [$tys.toArray,*]) : $ty → $ty
+      $rmapCases:matchAlt*
+    )
+
+    mkMapInstances .rmap
+    mkSuffixInstances .rmap
+    mkMapThms .rmap
+    mkFromActionMapThms .rmap
+
+    elabCommand $ ← `(
+      instance : RenMapEmpty $ty where
+        apply_empty := by intro $s:ident; simp [RenMap.rmap]
+
+      instance : RenMapId $ty [$ty] where
+        apply_id := by subst_solve_id
+
+      instance : RenMapCompose $ty [$ty] where
+        apply_compose := by subst_solve_compose
+    )
+
+    mkMapAllInstances .rmap
+
+    -- Executing smap stuff
+    let smapCases ← mkAllCases (map_f .smap false) tyNameGlobal (fVar := some $ smap_fVar tys)
+
+    elabCommand $ ← `(
+      @[simp]
+      def $smap ($σ : SubstVec [$tys.toArray,*]) : $ty → $ty
+      $smapCases:matchAlt*
+    )
+
+    mkMapInstances .smap
+    mkSuffixInstances .smap
+    mkMapAllInstances .smap
+    mkMapThms .smap
+    mkFromActionMapThms .smap
+
+    elabCommand $ ← `(
+      instance : SubstMapEmpty $ty where
+        apply_empty := by intro $s:ident; simp [SubstMap.smap]
+
+      instance : SubstMapId $ty [$ty] where
+        apply_id := by subst_solve_id
+
+      instance : SubstMapStable $ty [$ty] where
+        apply_stable := by subst_solve_stable
+
+      instance : SubstMapRenComposeLeft $ty [$ty] where
+        apply_ren_compose_left := by subst_solve_compose
+
+      instance : SubstMapRenComposeRight $ty [$ty] where
+        apply_ren_compose_right := by subst_solve_compose
+
+      instance : SubstMapCompose $ty [$ty] where
+        apply_compose := by subst_solve_compose
+    )
+
+  def genAllTys : List Ident → CommandElabM Unit
+  | [] => pure ()
+  | .cons ty tys => do
+    genAllTys tys
+    genTy (ty :: tys)
+
+  elab "#leansubst" &"generate" tys:ident,* : command =>
+    genAllTys tys.getElems.toList.reverse
+
+end Automation
